SemanticEquivalence/Equivalence/Expression.v
@@ -1,0 +1,63 @@
+From Coq Require Import List.
+Require Import SetsClass.SetsClass.
+
+Require Import SemanticEquivalence.Syntax.
+Require Import SemanticEquivalence.Representation.
+Require Import SemanticEquivalence.Denotational.Definition.
+Require Import SemanticEquivalence.Denotational.Expressions.
+Require Import SemanticEquivalence.SmallStep.Step.
+
+Local Open Scope Z.
+Local Open Scope sets.
+
+Module Equivalence_Expr.
+Import Representation Lang_WhileDCF.
+Import SetsNotation WhileDCF_Notation DntSem.
+Import DntSem_WhileDCF_Expr SmallStep_WhileDCF.
+
+Theorem eval_multistep_nrm : forall s e v,
+  Z_in_range v ->
+  (eval_r e).(nrm) s (word_from_Z v) ->
+  multistep_expr s e (EConst v).
+Proof.
+  intros.
+  unfold multistep_expr, clos_refl_trans.
+  sets_unfold.
+  exists 114514%nat.
+Admitted.
+
+Definition not_const (e : expr) :=
+  match e with
+  | EConst _ => False
+  | _ => True
+  end.
+
+Theorem eval_multistep_err : forall s e,
+  (eval_r e).(err) s ->
+  exists e',
+  not_const e' /\
+  multistep_expr s e e' /\
+  forall e'',
+  not (step_expr s e' e'').
+Proof.
+  intros.
+Admitted.
+
+Theorem multistep_eval_nrm : forall s e v,
+  Z_in_range v ->
+  multistep_expr s e (EConst v) ->
+  (eval_r e).(nrm) s (word_from_Z v).
+Proof.
+  intros.
+Admitted.
+
+Theorem multistep_eval_err : forall s e e',
+  not_const e' ->
+  multistep_expr s e e' ->
+  (forall e'', not (step_expr s e' e'')) ->
+  (eval_r e).(err) s.
+Proof.
+  intros.
+Admitted.
+
+End Equivalence_Expr.
