SemanticEquivalence/Equivalence/Statements.v
@@ -1,0 +1,129 @@
+From Coq Require Import List.
+Require Import SetsClass.SetsClass.
+
+Require Import SemanticEquivalence.Syntax.
+Require Import SemanticEquivalence.Representation.
+Require Import SemanticEquivalence.Denotational.Definition.
+Require Import SemanticEquivalence.Denotational.Expressions.
+Require Import SemanticEquivalence.Denotational.Statements.
+Require Import SemanticEquivalence.SmallStep.Step.
+
+Local Open Scope Z.
+Local Open Scope sets.
+
+Module Equivalence_Com.
+Import Representation Lang_WhileDCF.
+Import SetsNotation WhileDCF_Notation DntSem.
+Import DntSem_WhileDCF_Expr DntSem_WhileDCF_Com SmallStep_WhileDCF.
+
+Definition multistep_com_term (s' : state) (k : list com_context) : (state * com * list com_context) :=
+  (s', [[skip]], k).
+
+Definition not_multistep_com_term (k : list com_context) (p : state * com * list com_context) : Prop :=
+  match p with
+  | (_, [[skip]], k) => False
+  | _ => True
+  end.
+
+Lemma step_com_ctx (prog : program) : forall s s' c c' k1 k1' k2,
+  multistep_com prog (s, c, k1) (s', c', k1') ->
+  multistep_com prog (s, c, k1 ++ k2) (s', c', k1' ++ k2).
+Proof.
+  intros.
+  destruct H.
+  induction x.
+  - unfold nsteps in H; sets_unfold in H.
+    injection H; intros; subst.
+    unfold multistep_com, clos_refl_trans.
+    sets_unfold.
+    exists 0%nat; simpl; sets_unfold.
+    reflexivity.
+  - simpl in H.
+    sets_unfold in H.
+    destruct H, H, x0, p.
+Admitted.
+
+
+Definition com_equiv_nrm (prog : program) : forall s s' c,
+  (eval_com prog c).(nrm) s s' <->
+  forall k,
+  multistep_com prog (s, c, k) (s', [[skip]], k).
+Proof.
+  intros.
+Admitted.
+
+Definition com_equiv_brk (prog : program) : forall s s' c,
+  (eval_com prog c).(brk) s s' <->
+  forall k,
+  multistep_com prog (s, c, k) (s', [[break]], k).
+Proof.
+  intros.
+Admitted.
+
+Definition com_equiv_cnt (prog : program) : forall s s' c,
+  (eval_com prog c).(cnt) s s' <->
+  forall k,
+  multistep_com prog (s, c, k) (s', [[continue]], k).
+Proof.
+  intros.
+Admitted.
+
+Definition com_equiv_ret (prog : program) : forall s s' c,
+  (eval_com prog c).(ret) s s' <->
+  forall k,
+  multistep_com prog (s, c, k) (s', [[return]], k).
+Proof.
+  intros.
+Admitted.
+
+Definition com_equiv_err (prog : program) : forall s c,
+  (eval_com prog c).(err) s <->
+  exists x',
+  forall k x'',
+  not_multistep_com_term k x' /\
+  multistep_com prog (s, c, k) x' /\
+  not (multistep_com prog x' x'').
+Proof.
+  intros.
+Admitted.
+
+Definition com_equiv_inf (prog : program) : forall s c,
+  (eval_com prog c).(inf) s <->
+  forall x' k,
+  multistep_com prog (s, c, k) x' ->
+  exists x'',
+  multistep_com prog x' x''.
+Proof.
+  intros.
+Admitted.
+
+
+Theorem program_equiv_nrm (prog : program) : forall s s',
+  (eval_program prog).(nrm) s s' <->
+  multistep_com prog (prog_entry prog s) (multistep_com_term s' nil).
+Proof.
+  intros.
+Admitted.
+
+Theorem program_equiv_err (prog : program) : forall s,
+  (eval_program prog).(err) s <->
+  exists x',
+  not_multistep_com_term nil x' ->
+  multistep_com prog (prog_entry prog s) x' ->
+  forall x'',
+  not (step_com prog x' x'').
+Proof.
+  intros.
+Admitted.
+
+Theorem program_equiv_inf (prog : program) : forall s,
+  (eval_program prog).(inf) s <->
+  forall x',
+  multistep_com prog (prog_entry prog s) x' ->
+  exists x'',
+  multistep_com prog x' x''.
+Proof.
+  intros.
+Admitted.
+
+End Equivalence_Com.
